PoS/Protocol.v
@@ -3,21 +3,101 @@ Require Import ssreflect ssrbool ssrnat eqtype ssrfun seq.
 From mathcomp
 Require Import path.
 Require Import Eqdep pred prelude idynamic ordtype pcm finmap unionmap heap coding.
+Require Import Blockchain.
 Set Implicit Arguments.
 Unset Strict Implicit.
 Unset Printing Implicit Defensive.
 
 (* Implementation of PoS protocol as a STS *)
+Parameter GenesisBlock : Block.
+
 Definition nid := nat.
 Definition peers_t := seq nid.
 
 Inductive Message :=
   | NullMsg
-  | Addr of nid & peers_t
-  | Connect of nid.
+  | AddrMsg of nid & peers_t
+  | ConnectMsg of nid
+  | BlockMsg of Block
+  | TxMsg of Transaction
+  | InvMsg of nid & seq Hash
+  | GetDataMsg of nid & Hash.
+
+Module MsgEq.
+Definition eq_msg a b :=
+ match a, b with
+  | NullMsg, NullMsg => true
+  | NullMsg, _ => false
+  | AddrMsg idA prsA, AddrMsg idB prsB => (idA == idB) && (prsA == prsB)
+  | AddrMsg _ _, _ => false
+  | ConnectMsg idA, ConnectMsg idB => (idA == idB)
+  | ConnectMsg _, _ => false
+  | BlockMsg bA, BlockMsg bB => (bA == bB)
+  | BlockMsg _, _ => false
+  | TxMsg tA, TxMsg tB => (tA == tB)
+  | TxMsg _, _ => false
+  | InvMsg pA hA, InvMsg pB hB => (pA == pB) && (hA == hB)
+  | InvMsg _ _, _ => false
+  | GetDataMsg pA hA, GetDataMsg pB hB => (pA == pB) && (hA == hB)
+  | GetDataMsg _ _, _ => false
+  end.
+
+(* A lot of duplication in this proof; what can be done about it? *)
+Lemma eq_msgP : Equality.axiom eq_msg.
+Proof.
+move=> ma mb. rewrite/eq_msg.
+case: ma=>[|n p|n|b|t|p h|p h].
+- case: mb=>//[|n' p'|n'|b'|t'|p' h'|p' h']; do? [by constructor 2]; by constructor 1.
+- case: mb=>//[|n' p'|n'|b'|t'|p' h'|p' h']; do? [by constructor 2].
+  case B: ((n == n') && (p == p')).
+  - by case/andP: B=>/eqP<-/eqP<-; constructor 1.
+  by case/Bool.andb_false_elim: B=>B; constructor 2; case; move/eqP: B.
+- case: mb=>//[|n' p'|n'|b'|t'|p' h'|p' h']; do? [by constructor 2].
+  case B: (n == n'); first by case/eqP:B=><-; constructor 1.
+  by constructor 2; case=>E; subst n'; rewrite eqxx in B.
+- case: mb=>//[|n' p'|n'|b'|t'|p' h'|p' h']; do? [by constructor 2].
+  case B: (b == b'); first by case/eqP:B=><-; constructor 1.
+  by constructor 2; case=>E; subst b'; rewrite eqxx in B.
+- case: mb=>//[|n' p'|n'|b'|t'|p' h'|p' h']; do? [by constructor 2].
+  case B: (t == t'); first by case/eqP:B=><-; constructor 1.
+  by constructor 2; case=>E; subst t'; rewrite eqxx in B.
+- case: mb=>//[|n' p'|n'|b'|t'|p' h'|p' h']; do? [by constructor 2].
+  case B: ((p == p') && (h == h')).
+  - by case/andP: B=>/eqP<-/eqP<-; constructor 1.
+  by case/Bool.andb_false_elim: B=>B; constructor 2; case; move/eqP: B.
+(* This is literally copy-pasted from directly above; better way to do this? *)
+- case: mb=>//[|n' p'|n'|b'|t'|p' h'|p' h']; do? [by constructor 2].
+  case B: ((p == p') && (h == h')).
+  - by case/andP: B=>/eqP<-/eqP<-; constructor 1.
+  by case/Bool.andb_false_elim: B=>B; constructor 2; case; move/eqP: B.
+Qed.
+
+Canonical Msg_eqMixin := Eval hnf in EqMixin eq_msgP.
+Canonical Msg_eqType := Eval hnf in EqType Message Msg_eqMixin.
+End MsgEq.
+Export MsgEq.
 
 Record Packet := mkP {src: nid; dst: nid; msg: Message}.
 Definition NullPacket := mkP 0 0 NullMsg.
+
+Module PacketEq.
+Definition eq_pkt a b :=
+  ((src a) == (src b)) && ((dst a) == (dst b)) && ((msg a) == (msg b)).
+
+Lemma eq_pktP : Equality.axiom eq_pkt.
+Proof.
+case=>sa da ma [sb] db mb; rewrite/eq_pkt/=.
+case P1: (sa == sb)=>/=; last by constructor 2; case=>/eqP; rewrite P1.
+case P2: (da == db)=>/=; last by constructor 2; case=> _ /eqP; rewrite P2.
+case P3: (ma == mb)=>/=; last by constructor 2; case=> _ _ /eqP; rewrite P3.
+by constructor 1; move/eqP: P1=><-; move/eqP: P2=><-; move/eqP: P3=><-.
+Qed.
+
+Canonical Packet_eqMixin := Eval hnf in EqMixin eq_pktP.
+Canonical Packet_eqType := Eval hnf in EqType Packet Packet_eqMixin.
+End PacketEq.
+Export PacketEq.
+
 
 Definition ToSend := seq Packet.
 Definition emitZero : ToSend := [:: NullPacket].
@@ -35,22 +115,47 @@ Record State :=
   Node {
     id : nid;
     peers : peers_t;
+    blockTree : BlockTree;
+    txPool : TxPool;
   }.
 
-Definition Init (n : nid) : State := Node n [:: n].
+Definition Init (n : nid) : State := Node n [:: n] [:: GenesisBlock] [::].
 Lemma peers_uniq_init (n : nid) : uniq [::n]. Proof. done. Qed.
   
-
 Definition updS : State -> Message -> (State * ToSend) :=
   fun (st: State) (msg: Message) =>
     match st with
-    | Node n prs =>
+    | Node n prs bt pool =>
       match msg with
-      | Connect peer => pair (Node n (undup (peer :: prs))) emitZero
-      | Addr _ knownPeers =>
+      | ConnectMsg peer => pair (Node n (undup (peer :: prs)) bt pool) emitZero
+
+      | AddrMsg _ knownPeers =>
         let: newP := [seq x <- knownPeers | x \notin prs] in
-        let: connects := [seq mkP n p (Connect n) | p <- newP] in
-          pair (Node n (undup (prs ++ newP))) (emitMany(connects))
+        let: connects := [seq mkP n p (ConnectMsg n) | p <- newP] in
+        pair (Node n (undup (prs ++ newP)) bt pool) (emitMany(connects))
+
+      | BlockMsg b => pair (Node n prs (btExtend bt b) pool) emitZero
+
+      | TxMsg tx => pair (Node n prs bt (tpExtend pool tx)) emitZero
+
+      | InvMsg p peerHashes =>
+        let: ownHashes := [seq hashB b | b <- bt] ++ [seq hashT t | t <- pool] in
+        let: newH := [seq h <- peerHashes | h \notin ownHashes] in
+        let: gets := [seq mkP n p (GetDataMsg n h) | h <- newH] in
+        pair st (emitMany(gets))
+
+      | GetDataMsg p h =>
+        let: matchingBlocks := [seq b <- bt | (hashB b) == h] in
+        let: matchingTxs := [seq t <- pool | (hashT t) == h] in
+        match ohead matchingBlocks with
+        | Some(b) => pair st (emitOne(mkP n p (BlockMsg b)))
+        | _ =>
+          match ohead matchingTxs with
+          | Some (tx) => pair st (emitOne(mkP n p (TxMsg tx)))
+          | _ => pair st emitZero
+          end
+        end
+
       | _ => pair st emitZero
       end
     end.
@@ -59,21 +164,24 @@ Lemma upd_id_constant :
   forall (s1 : State) (m : Message), let: s2 := (updS s1 m).1 in
     id s1 = id s2.
 Proof.
-case=> n1 p1 []; by [].
+case=> n1 p1 b1 t1 []; do? by [].
+move=> p h. simpl. case exB: (ohead _). by [].
+case exT: (ohead _); by [].
 Qed.
 
 Lemma upd_peers_uniq :
   forall (s1 : State) (m : Message), let: s2 := (updS s1 m).1 in
     uniq (peers s1) -> uniq (peers s2).
 Proof.
-case=> n1 p1 [].
-- by [].
+case=> n1 p1 b1 t1 []; do? by [].
 - case=> [known | n2 known]; move=> UniqP1; by apply undup_uniq.
 - simpl. move=> n2 UniqP1. case B: (n2 \in p1).
   + by apply undup_uniq.
   + rewrite cons_uniq undup_id.
     * rewrite B. by [].
-    * by [].
+    * by  [].
+move=> p h. simpl. case exB: (ohead _). by [].
+case exT: (ohead _); by [].
 Qed.  
 
 
@@ -87,7 +195,7 @@ Lemma id_constant :
 Proof.
 move=> s1 s2.
 case.
-- move=> eq. rewrite eq. by  [].
+- move=> eq. rewrite eq. by [].
 - move=> m Us. rewrite Us. apply upd_id_constant.
 Qed.
 
@@ -100,5 +208,4 @@ case.
 - move=> eq. rewrite -eq. by [].
 - move=> m Us. rewrite Us. apply upd_peers_uniq. by [].
 Qed.
-
 End Node.
