PoS/Semantics.v
@@ -3,48 +3,13 @@ Require Import ssreflect ssrbool ssrnat eqtype ssrfun seq.
 From mathcomp
 Require Import path.
 Require Import Eqdep pred prelude idynamic ordtype pcm finmap unionmap heap coding. 
-Require Import Protocol.
+Require Import Protocol Blockchain.
 Set Implicit Arguments.
 Unset Strict Implicit.
 Unset Printing Implicit Defensive.
 
 
 (* Network semantics *)
-Section PacketEqType.
-
-Definition eqpkt a b :=
-  ((src a) == (src b)) && ((dst a) == (dst b)) &&
-  match (msg a), (msg b) with
-  | NullMsg, NullMsg => true
-  | NullMsg, _ => false
-  | Addr idA prsA, Addr idB prsB => (idA == idB) && (prsA == prsB)
-  | Addr _ _, _ => false
-  | Connect idA, Connect idB => (idA == idB)
-  | Connect _, _ => false
-  end.
-
-Lemma eqpktP : Equality.axiom eqpkt.
-Proof.
-case=>sa da ma [sb] db mb; rewrite/eqpkt/=.
-case P1: (sa == sb)=>/=; last by constructor 2; case=>/eqP; rewrite P1.
-case P2: (da == db)=>/=; last by constructor 2; case=> _ /eqP; rewrite P2.
-move/eqP: P1=>P1; move/eqP: P2=>P2; subst sb db.
-case: ma=>[|n p|n].
-- case: mb=>//[|n' p'|n']; do? [by constructor 2]; by constructor 1.  
-- case: mb=>//[|n' p'|n']; do? [by constructor 2].
-  case B: ((n == n') && (p == p')).
-  - by case/andP: B=>/eqP<-/eqP<-; constructor 1.
-  by case/Bool.andb_false_elim: B=>B; constructor 2; case; move/eqP: B.
-case: mb=>//[|n' p'|n']; do? [by constructor 2].
-case B: (n == n'); first by case/eqP:B=><-; constructor 1.
-by constructor 2; case=>E; subst n'; rewrite eqxx in B.
-Qed.
-
-Canonical Packet_eqMixin := Eval hnf in EqMixin eqpktP.
-Canonical Packet_eqType := Eval hnf in EqType Packet Packet_eqMixin.
-
-End PacketEqType.
-
 Definition PacketSoup := seq Packet.
 
 Definition StateMap := union_map [ordType of nid] State.
@@ -55,10 +20,10 @@ Record World :=
     inFlightMsgs : PacketSoup;
     }.
 
-Check dst.
-
 Inductive reliable_step (w w' : World) : Prop :=
-| step_msg (p : Packet) (st st' : State) (ms : ToSend) of
+| Idle of w = w'
+
+| Deliver (p : Packet) (st st' : State) (ms : ToSend) of
       p \in inFlightMsgs w &
       find (dst p) (localState w) = Some st &
       updS st (msg p) = (st', ms) &      
